common/StackADT.v
@@ -3302,68 +3302,72 @@ Program Definition inject_perm_all: InjectPerm :=
   |}.
 
 
+(* Definition same_head (P: perm_type) (m m': stack_adt) := *)
+(*   list_forall2 *)
+(*     (fun tf1 tf2 => *)
+(*        match tf1, tf2 with *)
+(*        | _, nil => True *)
+(*        | a::r, b::nil => a = b *)
+(*        | _, _ => False *)
+(*        end *)
+(*        /\ forall f1, In f1 tf1 -> has_perm_frame (injperm:=inject_perm_all) P inject_id f1 -> In f1 tf2 *)
+(*     ) *)
+(*     m m'. *)
+
 Definition same_head (P: perm_type) (m m': stack_adt) :=
   list_forall2
     (fun tf1 tf2 =>
-       match tf1, tf2 with
-       | _, nil => True
-       | a::r, b::nil => a = b
-       | _, _ => False
-       end
-       /\ forall f1, In f1 tf1 -> has_perm_frame (injperm:=inject_perm_all) P inject_id f1 -> In f1 tf2
+       (* match tf1, tf2 with *)
+       (* | _, nil => True *)
+       (* | a::r, b::nil => a = b *)
+       (* | _, _ => False *)
+       (* end *)
+       (forall f1, In f1 tf1 -> has_perm_frame (injperm:=inject_perm_all) P inject_id f1 -> In f1 tf2)
+       /\ (forall f1, In f1 tf2 -> In f1 tf1)
     )
     m m'.
-
-Lemma same_head_get_frame_info:
-  forall P s1 s2 (SH: same_head P s1 s2)
-    (ND: nodup s1)
-    b f (GFI: get_frame_info s2 b = Some f),
-    get_frame_info s1 b = Some f.
-Proof.
-  induction 1; simpl; intros; eauto.
-  inv ND.
-  repeat destr_in H.
-  - destr. eauto.
-  - destr_in GFI. easy.
-    rewrite pred_dec_false. eauto.
-    intro IFR; eapply H3 in IFR; eauto. apply IFR.
-    eapply get_frame_info_in_stack; eauto.
-  - destr_in GFI; eauto.
-    + rewrite pred_dec_true.
-      simpl in *.
-      destr_in GFI.
-      rewrite in_frames_cons in *. destruct i; auto; easy.
-    + rewrite pred_dec_false. eauto.
-      intro IFR.
-      eapply H3 in IFR; eauto. apply IFR.
-      eapply get_frame_info_in_stack; eauto.
-Qed.
-
-Lemma same_head_in_impl:
-  forall P s1 s2, same_head P s1 s2 -> forall b, in_stack s2 b -> in_stack s1 b.
-Proof.
-  induction 1; simpl; intros; rewrite ? in_stack_cons in *; eauto.
-  repeat destr_in H.
-  - destruct H1. easy. apply IHlist_forall2 in H; auto.
-  - rewrite in_frames_cons in *.
-    destruct H1; auto.
-    destruct H; auto.
-  - rewrite in_frames_cons in *.
-    destruct H1; auto.
-    destruct H; auto.
-    easy.
-Qed.
 
 Lemma same_head_in_stack':
   forall P s1 s2, same_head P s1 s2 -> forall b fi, in_stack' s2 (b,fi) -> in_stack' s1 (b,fi).
 Proof.
   induction 1; simpl; intros; eauto.
-  repeat destr_in H.
-  - destruct H1. easy. apply IHlist_forall2 in H; auto.
-  - destruct H1; auto. easy.
-  - simpl. destruct H1; auto.
-    destruct H; auto.
-    easy.
+  destruct H.
+  destruct H1; auto.
+  left.
+  rewrite in_frames'_rew in H1. destruct H1 as (fr & IFR & INb1).
+  apply H2 in INb1.
+  rewrite in_frames'_rew; eauto.
+Qed.
+
+Lemma same_head_get_frame_info:
+  forall P s1 s2 (SH: same_head P s1 s2)
+    (ND: nodup s1) (ND': Forall nodupt s1)
+    b f (GFI: get_frame_info s2 b = Some f),
+    get_frame_info s1 b = Some f.
+Proof.
+  intros.
+  apply get_assoc_spec in GFI.
+  destruct GFI as (fr & tf & INblocks & INtf & INS).
+  exploit same_head_in_stack'; eauto.
+  rewrite in_stack'_rew. eexists; split; eauto.
+  rewrite in_frames'_rew. eexists; split; eauto.
+  intro INS'.
+  clear INblocks INtf INS.
+  rewrite in_stack'_rew in INS'. setoid_rewrite in_frames'_rew in INS'.
+  destruct INS' as (ttf & (tfr & IFR & ITF) & INS).
+  eapply get_assoc_stack_lnr; eauto.
+Qed.
+
+Lemma same_head_in_impl:
+  forall P s1 s2, same_head P s1 s2 -> forall b, in_stack s2 b -> in_stack s1 b.
+Proof.
+  intros.
+  eapply in_stack_in_frames_ex in H0. destruct H0 as (tf & INS & IFRS).
+  eapply in_frames_in_frame_ex in IFRS. destruct IFRS as (fr & IFRS & IFR).
+  apply in_frame_info in IFR. destruct IFR as (fi & IFR).
+  eapply in_stack'_in_stack. eapply same_head_in_stack'; eauto.
+  rewrite in_stack'_rew. eexists; split; eauto.
+  rewrite in_frames'_rew. eexists; split; eauto.
 Qed.
 
 Lemma same_head_fap:
@@ -3372,10 +3376,11 @@ Lemma same_head_fap:
   exists f2, f2 @ s2 : i /\ (forall ff1, In ff1 f1 -> has_perm_frame (injperm:= inject_perm_all) P inject_id ff1 -> In ff1 f2).
 Proof.
   induction 1; simpl; intros; eauto.
+  destruct H.
   destruct i.
   - apply frame_at_pos_last in FAP1. subst.
     exists b1; split. constructor; reflexivity.
-    destruct H. apply H0.
+    auto.
   - apply frame_at_pos_cons_inv in FAP1.
     eapply IHSH in FAP1. destruct FAP1 as (f2 & FAP2 & PROP).
     exists f2; split. apply frame_at_pos_cons. auto. eauto. omega.
@@ -3408,7 +3413,7 @@ Lemma same_head_more_perm {injperm: InjectPerm}:
 Proof.
   induction 1; simpl; intros; constructor; auto.
   - destruct H; split; auto.
-    intros; eapply H0; eauto.
+    intros; eapply H; eauto.
     destruct H2 as (b & o & k & p & NONE & IFR & PERM & IPC).
     exists b, o, k, p; repeat split; eauto. eapply SAMEPERM; eauto.
     rewrite in_stack_cons; left.
@@ -3418,7 +3423,7 @@ Proof.
 Qed.
 
 Lemma public_stack_access_same_head:
-  forall s1 (ND: nodup s1) s2 P (SH: same_head P s1 s2) b lo hi
+  forall s1 (ND: nodup s1) (ND': Forall nodupt s1) s2 P (SH: same_head P s1 s2) b lo hi
          (PSA: public_stack_access s1 b lo hi),
     public_stack_access s2 b lo hi.
 Proof.
@@ -3430,35 +3435,25 @@ Definition stack_top_is_new s :=
   top_tframe_prop (fun tf => tf = nil) s.
 
 Lemma is_stack_top_same_head:
-  forall P s1 (WF: wf_stack P inject_id s1) (ND: nodup s1) s2 P2 (SH: same_head P2 s1 s2) b
+  forall P s1 (WF: wf_stack P inject_id s1) (ND: nodup s1) s2 (SH: same_head P s1 s2) b
          o k p (PERM: P b o k p)
          (IST: is_stack_top s1 b),
     is_stack_top s2 b \/ ~ in_stack s2 b.
 Proof.
   intros.
   inv SH. easy.
-  repeat destr_in H.
-  - right. intro IS. rewrite in_stack_cons in IS. destruct IS as [IFR|IS]. easy.
-    eapply same_head_in_impl in IS; eauto.
-    inv ND.
-    eapply H5 in IS; eauto.
-  - red in IST. simpl in IST.
-    left. assert (in_frame f0 b).
-    {
-      red. unfold get_frames_blocks in IST.  simpl in IST.
-      rewrite in_app in IST. destruct IST; auto.
-      rewrite concat_In in H. destruct H as (lb & INlb & INblocs).
-      exfalso. inv WF.
-      red in H3. simpl in H3.
-      eapply H3; eauto. unfold inject_id; congruence.
-      red. unfold get_frames_blocks. rewrite concat_In.  eexists; split. 2: apply INblocs. eauto.
-    }
-    red; simpl. unfold get_frames_blocks.
-    simpl. rewrite in_app. left; auto.
+  destruct H.
+  red in IST. simpl in IST.
+  change (in_frames a1 b) in IST.
+  left. red. simpl.
+  change (in_frames b1 b).
+  edestruct in_frames_in_frame_ex as (fr & IFRS & IFR). eauto.
+  eapply in_frame_in_frames; eauto. apply H; auto.
+  exists b, o, k, p; repeat split; auto. unfold inject_id; congruence.
 Qed.
 
 Lemma stack_access_same_head:
-  forall s1 P (ND: nodup s1) (WF: wf_stack P inject_id s1) s2 P2 (SH: same_head P2 s1 s2) b lo hi k p
+  forall s1 P (ND: nodup s1) (ND': Forall nodupt s1) (WF: wf_stack P inject_id s1) s2 (SH: same_head P s1 s2) b lo hi k p
          (R: forall o, (lo <= o < hi)%Z -> P b o k p)
          (SA: stack_access s1 b lo hi),
     stack_access s2 b lo hi.
@@ -3473,9 +3468,8 @@ Proof.
 Qed.
 
 Lemma stack_access_same_head_or_not_in_stack:
-  forall s1 P (ND: nodup s1) (WF: wf_stack P inject_id s1) s2 b
-         P2
-         (SH: same_head P2 s1 s2 \/ ~ in_stack s2 b) lo hi k p
+  forall s1 P (ND: nodup s1) (ND': Forall nodupt s1) (WF: wf_stack P inject_id s1) s2 b
+         (SH: same_head P s1 s2 \/ ~ in_stack s2 b) lo hi k p
          (R: forall o, (lo <= o < hi)%Z -> P b o k p)
          (SA: stack_access s1 b lo hi),
     stack_access s2 b lo hi.
@@ -3486,19 +3480,45 @@ Proof.
   right. red. destr. apply get_frame_info_in_stack in Heqo. congruence.          
 Qed.
 
+Lemma max_in_le:
+  forall l a i,
+    In a l ->
+    (a <= fold_right Z.max i l)%Z.
+Proof.
+  induction l; simpl; intros; eauto.
+  easy. destruct H; eauto. subst. apply Z.le_max_l.
+  apply Z.max_le_iff. right; eauto.
+Qed.
+
+Lemma max_sublist:
+  forall l1 l2 i,
+    (forall x, In x l1 -> In x l2) ->
+    (fold_right Z.max i l1 <= fold_right Z.max i l2)%Z.
+Proof.
+  induction l1; simpl; intros; eauto.
+  induction l2; simpl; intros; eauto. omega.
+  apply Z.max_le_iff. right. apply IHl2. easy.
+  apply Z.max_lub_iff. split.
+  apply max_in_le; auto.
+  apply IHl1. auto.
+Qed.
+
 Lemma same_head_size:
   forall P s1 s2,
     same_head P s1 s2 ->
     (size_stack s2 <= size_stack s1)%Z.
 Proof.
   induction 1; simpl; intros; rewrite ? size_stack_cons. omega.
-  repeat destr_in H.
-  - omega.
-  - generalize (size_frames_pos (f::l)).
-    change (size_frames nil) with 0%Z. omega.
-  - apply Z.add_le_mono. auto.
-    rewrite ! size_frames_cons.
-    apply Z.max_le_compat_l. apply size_frames_pos.
+  cut (size_frames b1 <= size_frames a1)%Z. omega.
+  apply max_sublist. setoid_rewrite in_map_iff.
+  intros x (x0 & EQ & IN). exists x0; split; auto. apply H. auto.
+Qed.
+
+Lemma same_head_refl:
+  forall P s,
+    same_head P s s.
+Proof.
+  induction s; simpl; intros; constructor; eauto.
 Qed.
 
 (* For use in Mach and Asm, the parent_sp pointer is now computed on the stack
